src/LeanEVM/Eval.lean
@@ -22,7 +22,8 @@ def dispatch (evm: Evm) : Bytecode -> Outcome
 | Bytecode.Div => DIV evm
 | Bytecode.Pop => POP evm
 | Bytecode.Dup n => DUP evm n
-| Bytecode.Push n => PUSH evm n
+| Bytecode.Push bs => PUSH evm bs
+| Bytecode.Invalid => Error InvalidOpcode
 
 -- Execute a sequence of zero or more bytecodes from a given state.
 @[simp]
@@ -52,20 +53,26 @@ by
   simp
 
 -- Executing DUP0 has the right effect
-example (evm:Evm): ∃evm', (eval [Push n, Dup_0] evm) = (Ok evm') :=
+example (evm:Evm): ∃evm', (eval [Push ns, Dup_1] evm) = (Ok evm') :=
 by
+  let n := u256.from_bytes ns;
   exists {stack := n::n::evm.stack}
   simp [*]
 
 -- Executing DUP1 has the right effect
-example (evm:Evm): ∃evm', (eval [Push n, Push m, Dup_1] evm) = (Ok evm') :=
+example (evm:Evm): ∃evm', (eval [Push ns, Push ms, Dup_2] evm) = (Ok evm') :=
 by
+  let n := u256.from_bytes ns;
+  let m := u256.from_bytes ms;
   exists {stack := n::m::n::evm.stack}
   simp [*]
 
 -- Executing DUP2 has the right effect
-example (evm:Evm): ∃evm', (eval [Push n, Push m, Push l, Dup_2] evm) = (Ok evm') :=
+example (evm:Evm): ∃evm', (eval [Push ns, Push ms, Push ls, Dup_3] evm) = (Ok evm') :=
 by
+  let n := u256.from_bytes ns;
+  let m := u256.from_bytes ms;
+  let l := u256.from_bytes ls;
   exists {stack := n::l::m::n::evm.stack}
   simp [*]  
   simp_arith
